Semantic preservation in progress, missing the fby case and history restriction

src/Lustre/Normalization/Correctness.v
@@ -139,10 +139,45 @@ Module Type CORRECTNESS
   Qed.
   Hint Resolve before_st_follows.
 
-  Definition valid_after {B} (l : list ident) (st : fresh_st B) :=
-    fresh_st_valid st /\ before_st l st.
+  (** ** Conservation of valid_after *)
 
-  (** ** Conservation of sem_exp *)
+  Definition valid_after {A B} (l : list (ident * A)) (st : fresh_st B) :=
+    fresh_st_valid st /\ before_st (List.map fst l) st.
+
+  Fact fresh_ident_valid_after {A B} : forall (l : list (ident * A)) (a : B) id st st',
+      fresh_ident a st = (id, st') ->
+      valid_after l st ->
+      valid_after l st'.
+  Proof.
+    intros l a id st st' Hfresh [Hvalid Hbef].
+    repeat constructor; eauto.
+  Qed.
+  Hint Resolve fresh_ident_valid_after.
+
+  Fact idents_for_anns_valid_after {A} : forall (l : list (ident * A)) anns ids st st',
+      idents_for_anns anns st = (ids, st') ->
+      valid_after l st ->
+      valid_after l st'.
+  Proof.
+    induction anns; intros ids st st' Hids Hvalid;
+      simpl in Hids; repeat inv_bind; eauto.
+  Qed.
+  Hint Resolve idents_for_anns_valid_after.
+
+  Fact normalize_reset_valid_after {A} : forall (l : list (ident * A)) e e' eqs' st st',
+      normalize_reset e st = (e', eqs', st') ->
+      valid_after l st ->
+      valid_after l st'.
+  Proof.
+    intros l e e' eqs' st st' Hnorm Hvalid.
+    destruct (normalize_reset_spec e) as [[? [? [? Hspec]]]|Hspec]; subst;
+      rewrite Hspec in Hnorm; clear Hspec; repeat inv_bind; auto.
+    destruct (List.hd _ _); simpl in *.
+    repeat inv_bind. eauto.
+  Qed.
+  Hint Resolve normalize_reset_valid_after.
+
+  (** Some additional stuff *)
 
   Fact idents_for_anns_NoDupMembers : forall anns ids st st',
       fresh_st_valid st ->
@@ -175,38 +210,214 @@ Module Type CORRECTNESS
     eapply NoDup_app_In; eauto.
   Qed.
 
+  Import Permutation.
+
+  Fact fresh_ident_dom {A B V} : forall (vars : list (ident * A)) H H' a id (v : V) (st st' : fresh_st B),
+      valid_after vars st ->
+      Env.dom H ((List.map fst vars)++(st_ids st)) ->
+      fresh_ident a st = (id, st') ->
+      H' = Env.add id v H ->
+      Env.dom H' ((List.map fst vars)++(st_ids st')).
+  Proof.
+    intros vars H H' a id v st st' Hvalid Hdom Hfresh Heq.
+    apply Facts.fresh_ident_vars_perm in Hfresh.
+    rewrite Heq.
+    apply Env.dom_add_cons with (x:=id) (v0:=v) in Hdom.
+    eapply Env.dom_Permutation; [| eauto].
+    symmetry. rewrite Permutation_middle.
+    apply Permutation_app_head. assumption.
+  Qed.
+
+  Fact fresh_ident_refines {A B V} : forall (vars : list (ident * A)) H H' a id (v : V) (st st' : fresh_st B),
+      valid_after vars st ->
+      Env.dom H ((List.map fst vars)++(st_ids st)) ->
+      fresh_ident a st = (id, st') ->
+      H' = Env.add id v H ->
+      Env.refines eq H H'.
+  Proof with eauto.
+    intros vars H H' a id v st st' Hvalid Hdom Hfresh Heq.
+    rewrite Heq.
+    assert (before_st (List.map fst vars) st') as Hbef1 by (destruct Hvalid as [_ ?]; eauto).
+    eapply Env.refines_add...
+    intro contra. erewrite Env.dom_use in contra; [| eauto].
+    apply in_app_or in contra. destruct contra.
+    + eapply Facts.fresh_ident_In in Hfresh.
+      assert (In id (st_ids st')).
+      { unfold st_ids, idty. repeat simpl_In; simpl in *.
+        exists (i, a); auto. }
+      apply smallest_ident_In in H1.
+      unfold before_st in Hbef1.
+      repeat rewrite_Forall_forall.
+      apply Hbef1 in H0.
+      apply (Pos.lt_irrefl id). eapply Pos.lt_le_trans...
+    + eapply Facts.fresh_ident_nIn in Hfresh. 2:(destruct Hvalid; eauto).
+      congruence.
+  Qed.
+
+  Fact idents_for_anns_dom {B V} : forall (vars : list (ident * B)) H H' anns ids (vs : list V) st st',
+      length vs = length ids ->
+      valid_after vars st ->
+      Env.dom H ((List.map fst vars)++(st_ids st)) ->
+      idents_for_anns anns st = (ids, st') ->
+      H' = Env.adds (List.map fst ids) vs H ->
+      Env.dom H' ((List.map fst vars)++(st_ids st')).
+  Proof with eauto.
+    intros vars H H' anns ids vs st st' Hlen Hvalid Hdom Hids Heq.
+    apply idents_for_anns_vars_perm in Hids.
+    rewrite Heq.
+    apply Env.dom_adds with (ids0:=List.map fst ids) (vs0:=vs) in Hdom.
+    2:(repeat rewrite_Forall_forall; solve_length).
+    eapply Env.dom_Permutation; [|eauto].
+    symmetry. rewrite Permutation_app_comm. rewrite <- app_assoc. apply Permutation_app_head.
+    rewrite Permutation_app_comm. assumption.
+  Qed.
+
+  Fact idents_for_anns_refines {B V} : forall (vars : list (ident * B)) H H' anns ids (vs : list V) st st',
+      length vs = length ids ->
+      valid_after vars st ->
+      Env.dom H ((List.map fst vars)++(st_ids st)) ->
+      idents_for_anns anns st = (ids, st') ->
+      H' = Env.adds (List.map fst ids) vs H ->
+      Env.refines eq H H'.
+  Proof with eauto.
+    intros vars H H' anns ids vs st st' Hlen Hvalid Hdom Hids Heq.
+    assert (Forall (fun id => ~List.In id (List.map fst vars)) (List.map fst ids)) as Hnvar.
+    { assert (valid_after vars st') by eauto.
+      apply idents_for_anns_incl in Hids.
+      solve_forall.
+      eapply incl_map in Hids. apply Hids in H1. clear Hids.
+      intro contra.
+      destruct H0 as [_ H0]. unfold before_st in H0.
+      rewrite Forall_forall in H0. apply H0 in contra.
+      unfold idty in H1. rewrite map_map in H1. simpl in H1.
+      apply smallest_ident_In in H1.
+      apply (Pos.lt_irrefl x). eapply Pos.lt_le_trans...
+    }
+    rewrite Heq. apply Env.refines_adds.
+    apply idents_for_anns_nIn in Hids; auto.
+    rewrite Forall_forall in *. intros x1 Hin contra.
+    erewrite Env.dom_use in contra; [|eauto].
+    apply in_app_or in contra; destruct contra.
+    + eapply Hnvar...
+    + eapply Hids...
+    + destruct Hvalid...
+  Qed.
+
+  (** ** Relation between state and history *)
+
+  (** We want to specify the semantics of the init equations created during the normalization
+      with idents stored in the env *)
+
+  Axiom init_stream : clock -> Stream OpAux.value.
+
+  Definition init_eqs_valids G b H st :=
+    Forall (fun '(id, (ty, cl, is_init)) =>
+                  is_init = true ->
+                  sem_equation G (Env.add id (init_stream (fst cl)) H)
+                               b ([id], [Efby [add_whens (Econst Op.true_const) ty (fst cl)]
+                                              [add_whens (Econst Op.false_const) ty (fst cl)] [(ty, cl)]])) (st_anns st).
+
+  Definition hist_st {A} G (l : list (ident * A)) b H st :=
+    Env.dom H ((List.map fst l)++(st_ids st)) /\
+    init_eqs_valids G b H st.
+
+  Fact fresh_ident_hist_st {A} : forall G (vars : list (ident * A)) b a id v H st st',
+      valid_after vars st ->
+      fresh_ident (a, false) st = (id, st') ->
+      hist_st G vars b H st ->
+      hist_st G vars b (Env.add id v H) st'.
+  Proof.
+    intros G vars b a id v H st st' Hvalid Hfresh [H1 H2].
+    constructor.
+    - eapply fresh_ident_dom; eauto.
+    - unfold init_eqs_valids in *.
+      assert (~In id (st_ids st)) by (destruct Hvalid; eapply Facts.fresh_ident_nIn in Hfresh; eauto).
+      assert (valid_after vars st') as Hvalid2 by eauto.
+      eapply fresh_ident_anns in Hfresh.
+      rewrite Hfresh.
+      constructor; eauto.
+      + destruct a. intros. congruence.
+      + repeat rewrite_Forall_forall.
+        destruct x as [id0 [[ty cl] is_init]].
+        specialize (H2 _ H3). simpl in H2.
+        intro His. apply H2 in His. clear H2.
+        eapply sem_equation_refines; [| eauto].
+        apply Env.refines_add_both; [| reflexivity].
+        eapply Env.refines_add. eauto.
+        intro contra.
+        erewrite Env.dom_use in contra; [| eauto].
+        eapply in_app_or in contra.
+        destruct contra.
+        * assert (In id (st_ids st')).
+          { unfold st_ids, idty. rewrite Hfresh. simpl. auto. }
+          eapply smallest_ident_In in H4.
+          destruct Hvalid2 as [_ Hvalid2].
+          unfold before_st in Hvalid2. rewrite Forall_forall in Hvalid2.
+          apply Hvalid2 in H2.
+          apply (Pos.lt_irrefl id).
+          eapply Pos.lt_le_trans; eauto.
+        * congruence.
+  Qed.
+  Hint Resolve fresh_ident_hist_st.
+
+  Fact idents_for_anns_hist_st {A} : forall G (vars : list (ident * A)) b anns ids vs H st st',
+      length vs = length ids ->
+      valid_after vars st ->
+      idents_for_anns anns st = (ids, st') ->
+      hist_st G vars b H st ->
+      hist_st G vars b (Env.adds (List.map fst ids) vs H) st'.
+  Proof with eauto.
+    intros G vars b anns ids vs H st st' Hlen Hvalid Hids Hist.
+    constructor.
+    - destruct Hist.
+      eapply idents_for_anns_dom in Hids...
+    - revert ids vs H st st' Hlen Hvalid Hids Hist.
+      induction anns; intros; simpl in Hids; repeat inv_bind; simpl.
+      + unfold Env.adds; simpl. destruct Hist. assumption.
+      + destruct vs; simpl in Hlen; try congruence.
+        unfold Env.adds; simpl.
+        assert (valid_after vars st') by eauto.
+        assert (valid_after vars x0) by eauto.
+        eapply fresh_ident_hist_st in H0...
+        eapply IHanns in H1...
+  Qed.
+  Hint Resolve idents_for_anns_hist_st.
+
+  (** ** Conservation of sem_exp *)
+
   Fact map_bind2_sem : forall G vars b is_control es H vs es' eqs' st st',
       Forall (wt_exp G vars) es ->
       Forall2 (sem_exp G H b) es vs ->
-      valid_after (List.map fst vars) st ->
-      Env.dom H ((List.map fst vars)++(st_ids st)) ->
+      valid_after vars st ->
+      hist_st G vars b H st ->
       Forall2 (fun e v => forall H es' eqs' st st',
                    sem_exp G H b e v ->
-                   valid_after (List.map fst vars) st ->
-                   Env.dom H ((List.map fst vars)++(st_ids st)) ->
+                   valid_after vars st ->
+                   hist_st G vars b H st ->
                    normalize_exp is_control e st = (es', eqs', st') ->
                    (exists H',
                        Env.refines eq H H' /\
-                       Env.dom H' ((List.map fst vars)++(st_ids st')) /\
+                       valid_after vars st' /\
+                       hist_st G vars b H' st' /\
                        Forall2 (fun e v => sem_exp G H' b e [v]) es' v /\
                        Forall (sem_equation G H' b) eqs')) es vs ->
       map_bind2 (normalize_exp is_control) es st = (es', eqs', st') ->
       (exists H',
           Env.refines eq H H' /\
-          Env.dom H' ((List.map fst vars)++(st_ids st')) /\
+          valid_after vars st' /\
+          hist_st G vars b H' st' /\
           Forall2 (fun es vs => Forall2 (fun e v => sem_exp G H' b e [v]) es vs) es' vs /\
           Forall (sem_equation G H' b) (concat eqs')).
   Proof with eauto.
-    induction es; intros H vs es' eqs' st st' Hwt Hsem Hbef Hdom Hf Hmap;
+    induction es; intros H vs es' eqs' st st' Hwt Hsem Hvalid Histst Hf Hmap;
       inv Hwt; inv Hsem; inv Hf; simpl in Hmap; repeat inv_bind.
-    - exists H; simpl. repeat split; auto.
-    - specialize (H7 _ _ _ _ _ H4 Hbef Hdom H0). destruct H7 as [H' [Href1 [Hdom1 [Hsem1 Hsem1']]]].
+    - exists H; simpl. repeat (split; eauto).
+    - specialize (H7 _ _ _ _ _ H4 Hvalid Histst H0). destruct H7 as [H' [Href1 [Hvalid1 [Histst1 [Hsem1 Hsem1']]]]].
       assert (Forall2 (sem_exp G H' b) es l') as Hsem'.
       { repeat rewrite_Forall_forall. eapply sem_exp_refines... }
-      assert (valid_after (List.map fst vars) x1) as Hbef1 by (destruct Hbef; constructor; eauto).
-      specialize (IHes _ _ _ _ _ _ H3 Hsem' Hbef1 Hdom1 H9 H1). clear H9.
-      destruct IHes as [H'' [Href2 [Hdom2 [Hsem2 Hsem2']]]].
-      exists H''. repeat split; simpl...
+      specialize (IHes _ _ _ _ _ _ H3 Hsem' Hvalid1 Histst1 H9 H1). clear H9.
+      destruct IHes as [H'' [Href2 [Hvalid2 [Histst2 [Hsem2 Hsem2']]]]].
+      exists H''. repeat (split; eauto).
       + etransitivity...
       + constructor; eauto. subst.
         specialize (normalize_exp_length _ _ _ _ _ _ _ _ H2 H0) as Hlength1.
@@ -218,69 +429,287 @@ Module Type CORRECTNESS
         solve_forall. eapply sem_equation_refines...
   Qed.
 
-  Import Permutation.
+  Fact normalize_reset_sem {B} : forall G (vars : list (ident * B)) b e H v e' eqs' st st',
+      sem_exp G H b e [v] ->
+      valid_after vars st ->
+      hist_st G vars b H st ->
+      Env.dom H ((List.map fst vars)++(st_ids st)) ->
+      normalize_reset e st = (e', eqs', st') ->
+      (exists H',
+          Env.refines eq H H' /\
+          valid_after vars st' /\
+          hist_st G vars b H' st' /\
+          sem_exp G H' b e' [v] /\
+          Forall (sem_equation G H' b) eqs').
+  Proof with eauto.
+    intros G vars b e H v e' eqs' st st' Hsem Hvalid Histst Hdom Hnorm.
+    specialize (normalize_reset_spec e) as [[? [? [? Hspec]]]|Hspec]; subst;
+      rewrite Hspec in Hnorm; clear Hspec; repeat inv_bind.
+    - exists H. repeat (split; auto).
+    - destruct (List.hd _ _) eqn:Heqann; simpl in *; repeat inv_bind.
+      assert (fresh_st_follows st st') as Hfollows by eauto.
+      assert (valid_after vars st') as Hvalid1 by eauto.
+      remember (Env.add x v H) as H'.
+      assert (hist_st G vars b H' st') by (subst; eauto).
+      assert (Env.refines eq H H') as Href by (eapply fresh_ident_refines with (st0:=st); eauto).
+      exists H'. repeat (split; eauto).
+      + constructor.
+        econstructor; [| reflexivity].
+        rewrite HeqH'. apply Env.add_1. reflexivity.
+      + repeat constructor.
+        apply Seq with (ss:=[[v]]).
+        * repeat constructor.
+          eapply sem_exp_refines...
+        * simpl. repeat constructor.
+          econstructor; [| reflexivity].
+          rewrite HeqH'. apply Env.add_1. reflexivity.
+  Qed.
+
+  Fact fby_iteexp_sem {B} : forall G (vars : list (ident * B)) b H e0 e a y0 y z e' eqs' st st',
+      sem_exp G H b e0 [y0] ->
+      sem_exp G H b e [y] ->
+      fby y0 y z ->
+      valid_after vars st ->
+      hist_st G vars b H st ->
+      fby_iteexp e0 e a st = (e', eqs', st') ->
+      (exists H',
+          Env.refines eq H H' /\
+          valid_after vars st' /\
+          hist_st G vars b H' st' /\
+          sem_exp G H' b e' [z] /\
+          Forall (sem_equation G H' b) eqs').
+  Proof with eauto.
+    intros G vars b H e0 e [ty cl] y0 y z e' eqs' st st' Hsem0 Hsem Hfby Hvalid Histst Hiteexp.
+    destruct (fby_iteexp_spec e0 e ty cl) as [[? [? Hspec]]|Hspec]; subst;
+      rewrite Hspec in Hiteexp; clear Hspec; repeat inv_bind.
+    - exists H. repeat (split; eauto).
+      econstructor.
+      + constructor; eauto.
+      + constructor; eauto.
+      + repeat constructor. assumption.
+    - unfold init_var_for_clock in H0.
+      destruct (find _ _) eqn:Hfind.
+      + destruct p; inv H0.
+        remember (Env.add x2 z H) as H'. (* z ? *)
+        assert (Env.refines eq H H') by (destruct Histst; eapply fresh_ident_refines in H1; eauto).
+        exists H'. repeat (split; eauto).
+        * destruct Histst. eapply fresh_ident_dom in H1...
+        * eapply fresh_ident_hist_st in H1...
+          rewrite <- HeqH' in H1.
+          destruct H1...
+        * (* We can get data about x back from our hist_st hypothesis *)
+          assert (sem_equation G (Env.add x (init_stream (fst cl)) H) b
+                               ([x], [Efby [add_whens (Econst Op.true_const) Op.bool_type (fst cl)]
+                                           [add_whens (Econst Op.false_const) Op.bool_type (fst cl)]
+                                           [(Op.bool_type, cl)]])) as Hsemx.
+          { destruct Histst as [_ Hvalids]. unfold init_eqs_valids in Hvalids.
+            rewrite Forall_forall in Hvalids.
+            eapply find_some in Hfind. destruct p as [[ty' cl'] isinit].
+            repeat rewrite Bool.andb_true_iff in Hfind. destruct Hfind as [Hin [[Hisinit Hcl] Hty]].
+            rewrite OpAux.type_eqb_eq in Hty.
+            rewrite Clocks.nclock_eqb_eq in Hcl. subst.
+            eapply Hvalids in Hin. apply Hin...
+          }
+          (* not exactly z *) admit.
+        * repeat constructor. (* idem *) admit.
+      + clear Hfind.
+        destruct (fresh_ident _ _) eqn:Hident. repeat inv_bind.
+        assert (valid_after vars x1) as Hvalid1 by eauto.
+        remember (Env.add x (init_stream (fst cl)) H) as H'.
+        assert (Env.refines eq H H') as Href1 by (destruct Histst; eapply fresh_ident_refines in Hident; eauto).
+        (* sem_exp (true fby false) init_stream *)
+        (* sem_equation H' ([x], [true fby false]) *)
+        assert (hist_st G vars b H' x1) as Histst1 by admit.
+        assert (valid_after vars st') as Hvalid2 by eauto.
+        remember (Env.add x2 z H') as H''.
+        assert (Env.refines eq H' H'') as Href2 by (destruct Histst1; eapply fresh_ident_refines in H1; eauto).
+        assert (hist_st G vars b H'' st') as Histst2 by (rewrite HeqH''; eauto).
+        assert (~Env.E.eq x2 x) as Hneq.
+        { intro contra. eapply Facts.fresh_ident_In in Hident.
+          assert (In x (st_ids x1)).
+          { unfold st_ids, idty. rewrite in_map_iff. exists (x, (Op.bool_type, cl, true)); eauto. }
+          eapply Facts.fresh_ident_nIn in H1. 2:(destruct Hvalid1; eauto).
+          rewrite contra in H1. congruence. }
+        exists H''. repeat (split; eauto)...
+        * etransitivity...
+        * eapply Site with (s:=(init_stream (fst cl))) (ts:=[[y0]]) (fs:=[[z]]).
+          -- constructor. econstructor; [| reflexivity].
+             rewrite HeqH''. rewrite HeqH'.
+             eapply Env.add_2... eapply Env.add_1. reflexivity.
+          -- repeat constructor.
+             eapply sem_exp_refines; [| eauto]. etransitivity...
+          -- repeat constructor. econstructor; [| reflexivity].
+             rewrite HeqH''. eapply Env.add_1. reflexivity.
+          -- simpl. repeat constructor.
+             admit. (* Dire des choses sur init_stream (Un bout d'intepreteur ?) *)
+        * repeat constructor.
+          -- apply Seq with (ss:=[[z]]); simpl.
+             ++ repeat constructor. admit. (* pas exactement z *)
+             ++ repeat constructor. admit. (* ce serait trop facile *)
+          -- apply Seq with (ss:=[[init_stream (fst cl)]]); simpl.
+             ++ admit.
+             ++ repeat constructor. econstructor; [| reflexivity].
+                rewrite HeqH''. rewrite HeqH'.
+                eapply Env.add_2... eapply Env.add_1. reflexivity.
+  Admitted.
+
+  Fact normalize_fby_sem {B} : forall G (vars : list (ident * B)) b anns H e0s es s0s ss vs es' eqs' st st',
+      length e0s = length anns ->
+      length es = length anns ->
+      Forall2 (fun e v => sem_exp G H b e [v]) e0s s0s ->
+      Forall2 (fun e v => sem_exp G H b e [v]) es ss ->
+      Forall3 fby s0s ss vs ->
+      valid_after vars st ->
+      hist_st G vars b H st ->
+      normalize_fby e0s es anns st = (es', eqs', st') ->
+      (exists H',
+          Env.refines eq H H' /\
+          valid_after vars st' /\
+          hist_st G vars b H' st' /\
+          Forall2 (fun e v => sem_exp G H' b e [v]) es' vs /\
+          Forall (sem_equation G H' b) eqs').
+  Proof with eauto.
+    induction anns; intros H e0s es s0s ss vs es' eqs' st st' Hlen1 Hlen2 Hsem1 Hsem2 Hfby Hvalid Histst Hnorm;
+      unfold normalize_fby in Hnorm; repeat inv_bind.
+    - destruct e0s; simpl in *; try congruence.
+      destruct es; simpl in *; try congruence.
+      repeat inv_bind. inv Hsem1. inv Hsem2. inv Hfby.
+      exists H. repeat (split; eauto); simpl...
+    - destruct e0s; simpl in *; try congruence.
+      destruct es; simpl in *; try congruence.
+      repeat inv_bind.
+      inv Hlen1. inv Hlen2. inv Hsem1. inv Hsem2. inv Hfby.
+      destruct a as [ty cl].
+      eapply fby_iteexp_sem in H0... destruct H0 as [H' [Hvalid1 [Href1 [Hdom1 [Hsem1 Hsem1']]]]].
+      assert (Forall2 (fun (e1 : exp) (v : Stream OpAux.value) => sem_exp G H' b e1 [v]) e0s l').
+      { repeat rewrite_Forall_forall; solve_length. eapply sem_exp_refines... } clear H8.
+      assert (Forall2 (fun (e1 : exp) (v : Stream OpAux.value) => sem_exp G H' b e1 [v]) es l'0).
+      { repeat rewrite_Forall_forall; solve_length. eapply sem_exp_refines... } clear H10.
+      assert (normalize_fby e0s es anns x2 = (x3, (concat x4), st')) as Hnorm.
+      { unfold normalize_fby. repeat inv_bind.
+        repeat eexists; try inv_bind; eauto. }
+      eapply IHanns in Hnorm... clear IHanns.
+      destruct Hnorm as [H'' [Hvalid2 [Href2 [Hdom2 [Hsem2 Hsem2']]]]].
+      eexists H''. repeat (split; eauto).
+      + etransitivity...
+      + constructor...
+        eapply sem_exp_refines...
+      + simpl. eapply Forall_app; split...
+        solve_forall. eapply sem_equation_refines...
+  Qed.
+
   Hint Constructors sem_exp.
   Fact normalize_exp_sem : forall G vars b e H vs is_control es' eqs' st st',
       wt_exp G vars e ->
       sem_exp G H b e vs ->
-      valid_after (List.map fst vars) st ->
-      Env.dom H ((List.map fst vars)++(st_ids st)) ->
+      valid_after vars st ->
+      hist_st G vars b H st ->
       normalize_exp is_control e st = (es', eqs', st') ->
       (exists H',
           Env.refines eq H H' /\
-          Env.dom H' ((List.map fst vars)++(st_ids st')) /\
+          valid_after vars st' /\
+          hist_st G vars b H' st' /\
           Forall2 (fun e v => sem_exp G H' b e [v]) es' vs /\
           Forall (sem_equation G H' b) eqs').
   Proof with eauto.
-    induction e using exp_ind2; intros Hi vs is_control es' eqs' st st' Hwt Hsem Hbef Hdom Hnorm;
+    induction e using exp_ind2; intros Hi vs is_control es' eqs' st st' Hwt Hsem Hvalid Histst Hnorm;
       inv Hwt; inv Hsem; simpl in Hnorm; repeat inv_bind.
     - (* const *)
-      exists Hi. repeat split...
+      exists Hi. repeat (split; eauto).
     - (* var *)
-      exists Hi. repeat split...
+      exists Hi. repeat (split; eauto).
     - (* unop *)
       specialize (Typ.normalize_exp_typeof _ _ _ _ _ _ _ _ H2 H) as Htypeof.
-      specialize (IHe _ _ _ _ _ _ _ H2 H9 Hbef Hdom H). destruct IHe as [Hi' [Href [Hdom' [Hsem Hsem']]]].
+      specialize (IHe _ _ _ _ _ _ _ H2 H9 Hvalid Histst H). destruct IHe as [Hi' [Hvalid1 [Href1 [Hdom1 [Hsem1 Hsem1']]]]].
       assert (numstreams e = 1) by (rewrite <- length_typeof_numstreams; rewrite H3; reflexivity).
       eapply normalize_exp_length in H... rewrite H0 in H.
-      repeat singleton_length. inv Hsem. clear H10.
+      repeat singleton_length. inv Hsem1. clear H10.
       exists Hi'.
-      repeat split...
+      repeat (split; eauto).
       repeat econstructor... congruence.
     - (* binop *)
       specialize (Typ.normalize_exp_typeof _ _ _ _ _ _ _ _ H3 H) as Htypeof1.
       specialize (Typ.normalize_exp_typeof _ _ _ _ _ _ _ _ H4 H0) as Htypeof2.
       assert (numstreams e1 = 1) by (rewrite <- length_typeof_numstreams; rewrite H15; reflexivity).
       assert (numstreams e2 = 1) by (rewrite <- length_typeof_numstreams; rewrite H16; reflexivity).
-      specialize (IHe1 _ _ _ _ _ _ _ H3 H10 Hbef Hdom H). destruct IHe1 as [Hi' [Href1 [Hdom1 [Hsem1 Hsem1']]]].
+      specialize (IHe1 _ _ _ _ _ _ _ H3 H10 Hvalid Histst H). destruct IHe1 as [Hi' [Href1 [Hvalid1 [Histst1 [Hsem1 Hsem1']]]]].
       eapply sem_exp_refines in H13; [| eauto].
-      assert (valid_after (List.map fst vars) x1) as Hbef1 by (destruct Hbef; constructor; eauto).
-      specialize (IHe2 _ _ _ _ _ _ _ H4 H13 Hbef1 Hdom1 H0). destruct IHe2 as [Hi'' [Href2 [Hdom2 [Hsem2 Hsem2']]]].
+      specialize (IHe2 _ _ _ _ _ _ _ H4 H13 Hvalid1 Histst1 H0). destruct IHe2 as [Hi'' [Href2 [Hvalid2 [Histst2 [Hsem2 Hsem2']]]]].
       eapply normalize_exp_length in H... rewrite H1 in H.
       eapply normalize_exp_length in H0... rewrite H2 in H0.
       repeat singleton_length; subst.
       inv Hsem1. inv Hsem2. clear H14 H19.
       rewrite H5 in H15; inv H15. rewrite H6 in H16; inv H16.
       exists Hi''.
-      repeat split...
-      repeat econstructor...
-      + apply Href1 in H. destruct H as [? [? H]]; subst.
-        apply Href2 in H. destruct H as [? [? H]]; subst...
+      repeat (split; eauto).
+      + etransitivity...
       + repeat econstructor...
         * eapply sem_exp_refines...
         * congruence.
         * congruence.
-      + rewrite Forall_app. split...
-        solve_forall. eapply sem_equation_refines...
+      + apply Forall_app. split; solve_forall...
+        eapply sem_equation_refines...
     - (* fby *)
-      admit.
+      specialize (map_bind2_normalize_exp_length _ _ _ _ _ _ _ _ H4 H1) as Hlength1.
+      specialize (map_bind2_normalize_exp_length _ _ _ _ _ _ _ _ H5 H2) as Hlength2.
+      eapply map_bind2_sem in H1... 2:(repeat rewrite_Forall_forall; eapply nth_In in H17; eauto). clear H.
+      destruct H1 as [H' [Href1 [Histst1 [Hdom1 [Hsem1 Hsem1']]]]]. apply Forall2_concat in Hsem1.
+      assert (Forall2 (sem_exp G H' b) es sss) as Hsem' by (repeat rewrite_Forall_forall; eapply sem_exp_refines; eauto).
+      eapply map_bind2_sem in H2... 2:(repeat rewrite_Forall_forall; eapply nth_In in H19; eauto). clear H0.
+      destruct H2 as [H'' [Hvalid2 [Href2 [Hdom2 [Hsem2 Hsem2']]]]]. apply Forall2_concat in Hsem2.
+      assert (Forall2 (fun (e : exp) (v : Stream OpAux.value) => sem_exp G H'' b e [v]) (concat x2) (concat s0ss)) as Hsem''.
+      { repeat rewrite_Forall_forall. eapply sem_exp_refines... }
+      specialize (idents_for_anns_length _ _ _ _ H9) as Hlength.
+      assert (length vs = length a) as Hlength'.
+      { repeat rewrite_Forall_forall. repeat simpl_length.
+        rewrite <- H13. erewrite <- map_length. rewrite H7. solve_length. }
+      eapply normalize_fby_sem in H3; solve_length...
+      2,3: (erewrite <- map_length; try rewrite H6; try rewrite H7; solve_length).
+      destruct H3 as [H''' [Href3 [Hvalid3 [Hdom3 [Hsem3 Hsem3']]]]].
+      remember (Env.adds (List.map fst x8) vs H''') as H''''.
+      assert (Env.refines eq H''' H'''') as Href4.
+      { destruct Hdom3. eapply idents_for_anns_refines... solve_length. }
+      assert (hist_st G vars b H'''' st') as Histst4.
+      { rewrite HeqH''''. eapply idents_for_anns_hist_st in H9... solve_length. }
+      exists H''''. repeat (split; eauto)...
+      * repeat (etransitivity; eauto).
+      * rewrite Forall2_map_1.
+        repeat rewrite_Forall_forall; solve_length.
+        destruct (nth _ x8 _) eqn:Hnth.
+        repeat constructor. econstructor; [| reflexivity].
+        destruct a0. rewrite split_nth in Hnth; inv Hnth.
+        rewrite split_map_fst.
+        apply Env.adds_MapsTo; solve_length.
+        rewrite <- fst_NoDupMembers.
+        destruct Hvalid3.
+        apply idents_for_anns_NoDupMembers in H9...
+      * repeat rewrite Forall_app. repeat split.
+        -- rewrite Forall_map.
+           eapply Forall2_combine'.
+           repeat rewrite_Forall_forall; solve_length.
+           destruct (nth _ x8 _) eqn:Hnth1.
+           econstructor.
+           ++ repeat constructor.
+              specialize (H0 b0 (Str.const b Op.false_const) _ _ _ H22 eq_refl eq_refl).
+              eapply sem_exp_refines...
+           ++ simpl. repeat constructor.
+              econstructor.
+              destruct a0. rewrite split_nth in Hnth1; inv Hnth1.
+              rewrite split_map_fst.
+              apply Env.adds_MapsTo; solve_length. 2:reflexivity.
+              rewrite <- fst_NoDupMembers.
+              destruct Hvalid3.
+              apply idents_for_anns_NoDupMembers in H9...
+        -- solve_forall. repeat (eapply sem_equation_refines; eauto).
+        -- solve_forall. repeat (eapply sem_equation_refines; eauto).
+        -- solve_forall. eapply sem_equation_refines...
     - (* when *)
       specialize (map_bind2_normalize_exp_length _ _ _ _ _ _ _ _ H4 H0) as Hlength.
       erewrite <- (map_length _ (annots es)) in Hlength. erewrite <- typesof_annots in Hlength.
       eapply map_bind2_sem in H0... 2: (repeat rewrite_Forall_forall; eapply nth_In in H8; eauto).
-      destruct H0 as [H' [Href [Hdom1 [Hsem1 Hsem2]]]].
+      destruct H0 as [H' [Hvalid1 [Href1 [Hdom1 [Hsem1 Hsem1']]]]].
       apply Forall2_concat in Hsem1.
-      exists H'. repeat split; simpl...
+      exists H'. repeat (split; simpl; eauto).
       rewrite Forall2_map_1.
       eapply Forall2_trans_ex in H13; [| eauto].
       apply Forall2_combine_lr with (zs:=(typesof es)) in H13; auto.
@@ -291,24 +720,14 @@ Module Type CORRECTNESS
       + simpl. repeat constructor...
     - (* merge *)
       specialize (sem_exps_numstreams _ _ _ _ _ _ H5 H15) as Hlength3.
-      assert (fresh_st_follows st x2) as Hfollows1.
-      { eapply map_bind2_st_follows in H1; eauto. solve_forall. }
-      assert (valid_after (List.map fst vars) x2) as Hbef1.
-      { destruct Hbef. constructor; eauto.
-        eapply map_bind2_st_valid; eauto. solve_forall. }
       eapply map_bind2_sem in H1... 2:(repeat rewrite_Forall_forall; eapply nth_In in H17; eauto). clear H.
-      destruct H1 as [H' [Href1 [Hdom1 [Hsem1 Hsem1']]]]. apply Forall2_concat in Hsem1.
+      destruct H1 as [H' [Href1 [Hvalid1 [Histst1 [Hsem1 Hsem1']]]]]. apply Forall2_concat in Hsem1.
       assert (Forall2 (sem_exp G H' b) efs fs) as Hsem' by (repeat rewrite_Forall_forall; eapply sem_exp_refines; eauto).
-      assert (fresh_st_follows x2 x5) as Hfollows2.
-      { eapply map_bind2_st_follows in H2; eauto. solve_forall. }
-      assert (valid_after (List.map fst vars) x5) as Hbef2.
-      { destruct Hbef1. constructor; eauto.
-        eapply map_bind2_st_valid; eauto. solve_forall. }
       eapply map_bind2_sem in H2... 2:(repeat rewrite_Forall_forall; eapply nth_In in H19; eauto). clear H0.
-      destruct H2 as [H'' [Href2 [Hdom2 [Hsem2 Hsem2']]]]. apply Forall2_concat in Hsem2.
+      destruct H2 as [H'' [Href2 [Hvalid2 [Histst2 [Hsem2 Hsem2']]]]]. apply Forall2_concat in Hsem2.
       destruct is_control; repeat inv_bind.
       + (* control *)
-        exists H''. repeat split; simpl...
+        exists H''. repeat (split; simpl; eauto).
         * etransitivity...
         * rewrite Forall2_map_1.
           repeat rewrite typesof_annots in H9.
@@ -329,35 +748,13 @@ Module Type CORRECTNESS
         specialize (idents_for_anns_length _ _ _ _ H) as Hlength.
         remember (Env.adds (List.map fst x0) vs H'') as H'''.
         assert (Env.refines eq H'' H''') as Href3.
-        { assert (Forall (fun id => ~List.In id (List.map fst vars)) (List.map fst x0)) as Hnvar.
-          { assert (valid_after (List.map fst vars) st') by (destruct Hbef2; constructor; eauto).
-            apply idents_for_anns_incl in H.
-            solve_forall.
-            eapply incl_map in H. apply H in H1. clear H.
-            intro contra.
-            destruct H0 as [_ H0]. unfold before_st in H0.
-            rewrite Forall_forall in H0. apply H0 in contra.
-            unfold idty in H1. rewrite map_map in H1. simpl in H1.
-            apply smallest_ident_In in H1.
-            apply (Pos.lt_irrefl x1). eapply Pos.lt_le_trans...
-          }
-          rewrite HeqH'''. apply Env.refines_adds.
-          apply idents_for_anns_nIn in H; auto.
-          rewrite Forall_forall in *. intros x1 Hin contra.
-          erewrite Env.dom_use in contra; [|eauto].
-          apply in_app_or in contra; destruct contra.
-          + eapply Hnvar...
-          + eapply H...
-          + destruct Hbef2... }
-        exists H'''. repeat split...
+        { destruct Histst2. eapply idents_for_anns_refines...
+          repeat rewrite_Forall_forall; solve_length. }
+        assert (hist_st G vars b H''' st') as Histst3.
+        { rewrite HeqH'''. eapply idents_for_anns_hist_st in H...
+          repeat rewrite_Forall_forall. solve_length. }
+        exists H'''. repeat (split; eauto).
         * repeat (etransitivity; eauto).
-        * apply idents_for_anns_vars_perm in H. (* Env.dom_Permutation *)
-          rewrite HeqH'''.
-          apply Env.dom_adds with (ids:=List.map fst x0) (vs0:=vs) in Hdom2.
-          2:(repeat rewrite_Forall_forall; solve_length).
-          eapply Env.dom_Permutation; [|eauto].
-          symmetry. rewrite Permutation_app_comm. rewrite <- app_assoc. apply Permutation_app_head.
-          rewrite Permutation_app_comm. assumption.
         * rewrite Forall2_map_1.
           repeat rewrite_Forall_forall; solve_length.
           destruct (nth _ x0 _) eqn:Hnth.
@@ -366,7 +763,7 @@ Module Type CORRECTNESS
           rewrite split_map_fst.
           apply Env.adds_MapsTo; solve_length.
           rewrite <- fst_NoDupMembers.
-          destruct Hbef2.
+          destruct Hvalid2.
           apply idents_for_anns_NoDupMembers in H...
         * repeat rewrite Forall_app. repeat split.
           -- rewrite map_map; simpl.
@@ -396,7 +793,7 @@ Module Type CORRECTNESS
                 rewrite split_map_fst.
                 apply Env.adds_MapsTo; solve_length. 2:reflexivity.
                 rewrite <- fst_NoDupMembers.
-                destruct Hbef2.
+                destruct Hvalid2.
                 apply idents_for_anns_NoDupMembers in H...
           -- solve_forall. repeat (eapply sem_equation_refines; eauto).
           -- solve_forall. eapply sem_equation_refines...
@@ -405,29 +802,16 @@ Module Type CORRECTNESS
       specialize (sem_exp_numstreams _ _ _ _ _ _ H5 H14) as Hlength1. simpl in Hlength1.
       specialize (normalize_exp_length _ _ _ _ _ _ _ _ H5 H1) as Hlength1'. rewrite <- Hlength1 in Hlength1'. clear Hlength1.
       specialize (sem_exps_numstreams _ _ _ _ _ _ H6 H16) as Hlength3.
-      assert (fresh_st_follows st x1) as Hfollows1 by eauto.
-      assert (valid_after (List.map fst vars) x1) as Hbef1.
-      { destruct Hbef. constructor; eauto. }
-      eapply IHe in H1... clear IHe. destruct H1 as [H' [Href1 [Hdom1 [Hsem1 Hsem1']]]].
-      assert (fresh_st_follows x1 x4) as Hfollows2.
-      { eapply map_bind2_st_follows in H2; eauto. solve_forall. }
-      assert (valid_after (List.map fst vars) x4) as Hbef2.
-      { destruct Hbef1. constructor; eauto.
-        eapply map_bind2_st_valid; eauto. solve_forall. }
+      eapply IHe in H1... clear IHe. destruct H1 as [H' [Href1 [Hvalid1 [Histst1 [Hsem1 Hsem1']]]]].
       assert (Forall2 (sem_exp G H' b) ets ts) as Hsem' by (repeat rewrite_Forall_forall; eapply sem_exp_refines; eauto).
       eapply map_bind2_sem in H2... 2:(repeat rewrite_Forall_forall; eapply nth_In in H22; eauto). clear H.
-      destruct H2 as [H'' [Href2 [Hdom2 [Hsem2 Hsem2']]]]. apply Forall2_concat in Hsem2.
-      assert (fresh_st_follows x4 x7) as Hfollows3.
-      { eapply map_bind2_st_follows in H3; eauto. solve_forall. }
-      assert (valid_after (List.map fst vars) x7) as Hbef3.
-      { destruct Hbef2. constructor; eauto.
-        eapply map_bind2_st_valid; eauto. solve_forall. }
+      destruct H2 as [H'' [Href2 [Hvalid2 [Histst2 [Hsem2 Hsem2']]]]]. apply Forall2_concat in Hsem2.
       assert (Forall2 (sem_exp G H'' b) efs fs) as Hsem'' by (repeat rewrite_Forall_forall; repeat (eapply sem_exp_refines; eauto)).
       eapply map_bind2_sem in H3... 2:(repeat rewrite_Forall_forall; eapply nth_In in H24; eauto). clear H0.
-      destruct H3 as [H''' [Href3 [Hdom3 [Hsem3 Hsem3']]]]. apply Forall2_concat in Hsem3.
+      destruct H3 as [H''' [Href3 [Hvalid3 [Histst3 [Hsem3 Hsem3']]]]]. apply Forall2_concat in Hsem3.
       destruct is_control; repeat inv_bind.
       + (* control *)
-        exists H'''. repeat split; simpl...
+        exists H'''. repeat (split; simpl; eauto).
         * repeat (etransitivity; eauto).
         * rewrite Forall2_map_1.
           repeat rewrite typesof_annots in H10.
@@ -451,35 +835,13 @@ Module Type CORRECTNESS
         specialize (idents_for_anns_length _ _ _ _ H) as Hlength.
         remember (Env.adds (List.map fst x2) vs H''') as H''''.
         assert (Env.refines eq H''' H'''') as Href4.
-        { assert (Forall (fun id => ~List.In id (List.map fst vars)) (List.map fst x2)) as Hnvar.
-          { assert (valid_after (List.map fst vars) st') by (destruct Hbef3; constructor; eauto).
-            apply idents_for_anns_incl in H.
-            solve_forall.
-            eapply incl_map in H. apply H in H1. clear H.
-            intro contra.
-            destruct H0 as [_ H0]. unfold before_st in H0.
-            rewrite Forall_forall in H0. apply H0 in contra.
-            unfold idty in H1. rewrite map_map in H1. simpl in H1.
-            apply smallest_ident_In in H1.
-            apply (Pos.lt_irrefl x3). eapply Pos.lt_le_trans...
-          }
-          rewrite HeqH''''. apply Env.refines_adds.
-          apply idents_for_anns_nIn in H; auto.
-          rewrite Forall_forall in *. intros x3 Hin contra.
-          erewrite Env.dom_use in contra; [|eauto].
-          apply in_app_or in contra; destruct contra.
-          + eapply Hnvar...
-          + eapply H...
-          + destruct Hbef3... }
-        exists H''''. repeat split...
+        { destruct Histst3. eapply idents_for_anns_refines...
+          repeat rewrite_Forall_forall; solve_length. }
+        assert (hist_st G vars b H'''' st').
+        { rewrite HeqH''''. eapply idents_for_anns_hist_st in H...
+          repeat rewrite_Forall_forall. solve_length. }
+        exists H''''. repeat (split; eauto)...
         * repeat (etransitivity; eauto).
-        * apply idents_for_anns_vars_perm in H. (* Env.dom_Permutation *)
-          rewrite HeqH''''.
-          apply Env.dom_adds with (ids:=List.map fst x2) (vs0:=vs) in Hdom3.
-          2:(repeat rewrite_Forall_forall; solve_length).
-          eapply Env.dom_Permutation; [|eauto].
-          symmetry. rewrite Permutation_app_comm. rewrite <- app_assoc. apply Permutation_app_head.
-          rewrite Permutation_app_comm. assumption.
         * rewrite Forall2_map_1.
           repeat rewrite_Forall_forall; solve_length.
           destruct (nth _ x2 _) eqn:Hnth.
@@ -488,7 +850,7 @@ Module Type CORRECTNESS
           rewrite split_map_fst.
           apply Env.adds_MapsTo; solve_length.
           rewrite <- fst_NoDupMembers.
-          destruct Hbef3.
+          destruct Hvalid3.
           apply idents_for_anns_NoDupMembers in H...
         * repeat rewrite Forall_app. repeat split.
           -- rewrite map_map; simpl.
@@ -504,13 +866,11 @@ Module Type CORRECTNESS
                 ** simpl in H15. repeat singleton_length; subst.
                    eapply sem_exp_refines; [| eauto].
                    etransitivity... etransitivity...
-                ** rewrite_Forall_forall.
-                   simpl in H25. destruct n0; simpl; try omega.
-                   specialize (H9 e2 s _ _ _ H24 eq_refl eq_refl).
+                ** repeat constructor.
+                   specialize (H12 e2 s _ _ _ H25 eq_refl eq_refl).
                    eapply sem_exp_refines; [| eauto]. etransitivity...
-                ** rewrite_Forall_forall.
-                   simpl in H25. destruct n0; simpl; try omega.
-                   specialize (H9 e2 s _ _ _ H24 eq_refl eq_refl).
+                ** repeat constructor.
+                   specialize (H12 e2 s _ _ _ H25 eq_refl eq_refl).
                    eapply sem_exp_refines; [| eauto]. etransitivity...
                 ** repeat econstructor. eauto.
              ++ simpl. repeat constructor.
@@ -519,45 +879,468 @@ Module Type CORRECTNESS
                 rewrite split_map_fst.
                 apply Env.adds_MapsTo; solve_length. 2:reflexivity.
                 rewrite <- fst_NoDupMembers.
-                destruct Hbef3.
+                destruct Hvalid3.
                 apply idents_for_anns_NoDupMembers in H...
           -- solve_forall. repeat (eapply sem_equation_refines; eauto).
           -- solve_forall. eapply sem_equation_refines with (H:=H'')... etransitivity...
+          -- solve_forall. eapply sem_equation_refines...
              Unshelve. exact default_ann. exact (hd_default []). 1,2:exact s.
-  Admitted.
+    - (* app *)
+      specialize (idents_for_anns_length _ _ _ _ H2) as Hlength1.
+      assert (length (n_out n) = length vs) as Hlength2.
+      { destruct H14. repeat rewrite_Forall_forall.
+        rewrite H4 in H6. inv H6. unfold idents in *. solve_length. }
+      eapply map_bind2_sem in H1... 2:(repeat rewrite_Forall_forall; eapply nth_In in H12; eauto). clear H0.
+      destruct H1 as [H' [Href1 [Hvalid1 [Histst1 [Hsem1 Hsem1']]]]].
+      remember (Env.adds (List.map fst x3) vs H') as H''.
+      assert (Env.refines eq H' H'') as Href2.
+      { destruct Histst1.
+        eapply idents_for_anns_refines... repeat rewrite_Forall_forall; solve_length. }
+      assert (hist_st G vars b H'' st').
+      { rewrite HeqH''. eapply idents_for_anns_hist_st in H2...
+        repeat rewrite_Forall_forall. solve_length. }
+      exists H''. repeat (split; eauto).
+      + etransitivity...
+      + rewrite Forall2_map_1.
+        repeat rewrite_Forall_forall; solve_length.
+        destruct (nth _ x3 _) eqn:Hnth.
+        repeat constructor. econstructor; [|reflexivity].
+        destruct a1. rewrite split_nth in Hnth; inv Hnth.
+        rewrite split_map_fst.
+        apply Env.adds_MapsTo; solve_length.
+        rewrite <- fst_NoDupMembers.
+        destruct Hvalid1.
+        apply idents_for_anns_NoDupMembers in H2...
+      + constructor.
+        * apply Seq with (ss:=[vs]).
+          -- repeat constructor.
+             apply Sapp with (ss:=(concat (List.map (fun x => List.map (fun x => [x]) x) ss))).
+             ++ apply Forall2_concat.
+                repeat rewrite_Forall_forall; solve_length;
+                  specialize (H3 a0 (List.map (fun _ => (Str.const b (Op.false_const))) b0) _ _ _ H13 eq_refl eq_refl);
+                  repeat rewrite_Forall_forall; simpl_length.
+                ** rewrite <- map_nth.
+                   rewrite <- (map_nth (length (A:=_)) (List.map _ ss)). f_equal; solve_length.
+                   repeat rewrite map_map.
+                   apply map_ext_in. intros; solve_length.
+                ** specialize (H16 a1 (Str.const b (Op.false_const)) _ _ _ H15 eq_refl eq_refl).
+                   repeat simpl_nth; [| eassumption].
+                   eapply sem_exp_refines...
+             ++ rewrite concat_map_singl2. assumption.
+          -- simpl. rewrite app_nil_r.
+             repeat rewrite_Forall_forall; solve_length.
+             repeat constructor. econstructor; [| reflexivity].
+             apply Env.adds_MapsTo; solve_length.
+             rewrite <- fst_NoDupMembers.
+             destruct Hvalid1.
+             apply idents_for_anns_NoDupMembers in H2...
+        * solve_forall.
+          eapply sem_equation_refines...
+    - (* app (reset) *)
+      specialize (idents_for_anns_length _ _ _ _ H3) as Hlength1.
+      assert (length (n_out n) = length vs) as Hlength3.
+      { clear H H0 H1 H4. specialize (H19 0); inv H19; subst.
+        repeat rewrite_Forall_forall.
+        rewrite H0 in H6; inv H6. unfold idents in *. solve_length. }
+      assert (length x2 = 1) as Hlength2.
+      { eapply normalize_exp_length in H1... rewrite <- length_typeof_numstreams in H1.
+        rewrite H1. rewrite H11. reflexivity. }
+      repeat singleton_length; subst.
+      eapply H in H1... clear H.
+      destruct H1 as [H' [Href1 [Hvalid1 [Histst1 [Hsem1 Hsem1']]]]]. inv Hsem1; inv H16.
+      eapply normalize_reset_sem in H4... 2:(destruct Histst1; eauto).
+      destruct H4 as [H'' [Href2 [Hvalid2 [Histst2 [Hsem2 Hsem2']]]]].
+      assert (Forall2 (sem_exp G H'' b) es ss) as Hsem'.
+      { repeat rewrite_Forall_forall.
+        eapply sem_exp_refines; [| eauto]. etransitivity... } clear H15.
+      eapply map_bind2_sem in H2... 2:(repeat rewrite_Forall_forall; eapply nth_In in H14; eauto). clear H0.
+      destruct H2 as [H''' [Href3 [Hvalid3 [Histst3 [Hsem3 Hsem3']]]]].
+      remember (Env.adds (List.map fst x5) vs H''') as H''''.
+      assert (Env.refines eq H''' H'''') as Href4.
+      { destruct Histst3. eapply idents_for_anns_refines...
+        repeat rewrite_Forall_forall; solve_length. }
+      assert (valid_after vars st') as Hvalid4 by eauto.
+      assert (hist_st G vars b H'''' st').
+      { rewrite HeqH''''. eapply idents_for_anns_hist_st in H3...
+        repeat rewrite_Forall_forall; solve_length. }
+      exists H''''. repeat (split; auto).
+      + repeat (etransitivity; eauto).
+      + rewrite Forall2_map_1.
+        repeat rewrite_Forall_forall; solve_length.
+        destruct (nth _ x5 _) eqn:Hnth.
+        repeat constructor. econstructor; [|reflexivity].
+        destruct a1. rewrite split_nth in Hnth; inv Hnth.
+        rewrite split_map_fst.
+        apply Env.adds_MapsTo; solve_length.
+        rewrite <- fst_NoDupMembers.
+        destruct Hvalid3.
+        apply idents_for_anns_NoDupMembers in H3...
+      + constructor.
+        * apply Seq with (ss:=[vs]).
+          -- repeat constructor.
+             apply Sreset with (ss:=(concat (List.map (fun x => List.map (fun x => [x]) x) ss))) (rs:=rs) (bs:=bs)...
+             ++ apply Forall2_concat.
+                repeat rewrite_Forall_forall; solve_length;
+                  specialize (H1 a0 (List.map (fun _ => (Str.const b (Op.false_const))) b0) _ _ _ H15 eq_refl eq_refl);
+                  repeat rewrite_Forall_forall; simpl_length.
+                ** rewrite <- map_nth.
+                   rewrite <- (map_nth (length (A:=_)) (List.map _ ss)). f_equal; solve_length.
+                   repeat rewrite map_map.
+                   apply map_ext_in. intros; solve_length.
+                ** specialize (H20 a1 (Str.const b (Op.false_const)) _ _ _ H16 eq_refl eq_refl).
+                   repeat simpl_nth; [| eassumption].
+                   eapply sem_exp_refines...
+             ++ eapply sem_exp_refines; [| eauto]. etransitivity...
+             ++ rewrite concat_map_singl2. assumption.
+          -- simpl. rewrite app_nil_r.
+             repeat rewrite_Forall_forall; solve_length.
+             repeat constructor. econstructor; [| reflexivity].
+             apply Env.adds_MapsTo; solve_length.
+             rewrite <- fst_NoDupMembers.
+             destruct Hvalid3.
+             apply idents_for_anns_NoDupMembers in H3...
+        * repeat rewrite Forall_app.
+          repeat split; solve_forall; solve_length.
+          1,2,3: (eapply sem_equation_refines; [| eauto]; repeat (etransitivity; eauto)).
+  Qed.
+
+  Corollary normalize_exps_sem : forall G vars b es H vs es' eqs' st st',
+      Forall (wt_exp G vars) es ->
+      Forall2 (sem_exp G H b) es vs ->
+      valid_after vars st ->
+      hist_st G vars b H st ->
+      map_bind2 (normalize_exp false) es st = (es', eqs', st') ->
+      (exists H',
+          Env.refines eq H H' /\
+          valid_after vars st' /\
+          hist_st G vars b H' st' /\
+          Forall2
+            (fun (es : list exp) (vs : list (Stream OpAux.value)) =>
+             Forall2 (fun e v => sem_exp G H' b e [v]) es vs) es' vs /\
+          Forall (sem_equation G H' b) (concat eqs')).
+  Proof.
+    intros G vars b es H vs es' eqs' st st' Hwt Hsem Hvalid Hdom Hnorm.
+    eapply map_bind2_sem in Hnorm; eauto.
+    repeat rewrite_Forall_forall.
+    specialize (nth_In _ a H2) as Hin.
+    eapply normalize_exp_sem with (e:=(nth n es a)); eauto.
+  Qed.
+
+  Fact normalize_rhs_sem : forall G vars b keep_fby e H vs es' eqs' st st',
+      wt_exp G vars e ->
+      sem_exp G H b e vs ->
+      valid_after vars st ->
+      hist_st G vars b H st ->
+      normalize_rhs keep_fby e st = (es', eqs', st') ->
+      (exists H',
+          Env.refines eq H H' /\
+          valid_after vars st' /\
+          hist_st G vars b H' st' /\
+          (Forall2 (fun e v => sem_exp G H' b e [v]) es' vs \/
+           exists e', (es' = [e'] /\ sem_exp G H' b e' vs)) /\
+          Forall (sem_equation G H' b) eqs').
+  Proof with eauto.
+    intros G vars b keep_fby e H vs es' eqs' st st' Hwt Hsem Hvalid Hhistst Hnorm.
+    destruct e; try eapply normalize_exp_sem in Hnorm; eauto.
+    1,2,3,4,6,7,8: (destruct Hnorm as [H' [Href1 [Hvalid1 [Hhistst1 [Hsem1 Hsem2]]]]];
+                    exists H'; repeat (split; eauto)).
+      1,2:(unfold normalize_rhs in Hnorm). destruct keep_fby. 1,2,3:(inv Hwt; inv Hsem).
+    - (* fby (keep) *)
+      repeat inv_bind.
+      specialize (normalize_exps_length _ _ _ _ _ _ _ H3 H0) as Hlength2.
+      specialize (normalize_exps_length _ _ _ _ _ _ _ H4 H1) as Hlength1.
+      unfold normalize_exps in *. repeat inv_bind.
+      eapply normalize_exps_sem in H0...
+      destruct H0 as [H' [Href1 [Hvalid1 [Histst1 [Hsem1 Hsem1']]]]]. apply Forall2_concat in Hsem1.
+      assert (Forall2 (sem_exp G H' b) l0 sss) as Hsem' by (repeat rewrite_Forall_forall; eapply sem_exp_refines; eauto).
+      eapply normalize_exps_sem in H1...
+      destruct H1 as [H'' [Href2 [Hvalid2 [Histst2 [Hsem2 Hsem2']]]]]. apply Forall2_concat in Hsem2.
+      assert (Forall2 (fun (e : exp) (v : Stream OpAux.value) => sem_exp G H'' b e [v]) (concat x2) (concat s0ss)) as Hsem''.
+      { repeat rewrite_Forall_forall. eapply sem_exp_refines... }
+      eapply normalize_fby_sem in H2; solve_length...
+      2,3: (erewrite <- map_length; try rewrite H5; try rewrite H6; solve_length).
+      destruct H2 as [H''' [Href3 [Hvalid3 [Histst3 [Hsem3 Hsem3']]]]].
+      exists H'''. repeat (split; auto).
+      + repeat (etransitivity; eauto).
+      + repeat rewrite Forall_app. repeat split...
+        * solve_forall. eapply sem_equation_refines; [| eauto]. etransitivity...
+        * solve_forall. eapply sem_equation_refines...
+    - (* fby (don't keep) *)
+      eapply normalize_exp_sem in Hnorm...
+      destruct Hnorm as [H' [Href1 [Hvalid1 [Histst1 [Hsem1 Hsem2]]]]].
+      exists H'. repeat (split; eauto).
+    - (* app *)
+      repeat inv_bind. unfold normalize_exps in H0; repeat inv_bind.
+      eapply normalize_exps_sem in H0...
+      destruct H0 as [H' [Href1 [Hvalid1 [Histst1 [Hsem1 Hsem1']]]]].
+      exists H'. repeat (split; auto).
+      right. eexists; split...
+      apply Sapp with (ss:=(concat (List.map (fun x => List.map (fun x => [x]) x) ss))).
+      * apply Forall2_concat.
+        repeat rewrite_Forall_forall; solve_length;
+          specialize (H1 a (List.map (fun _ => (Str.const b (Op.false_const))) b0) _ _ _ H11 eq_refl eq_refl);
+          repeat rewrite_Forall_forall; simpl_length.
+        -- rewrite <- map_nth.
+           rewrite <- (map_nth (length (A:=_)) (List.map _ ss)). f_equal; solve_length.
+           repeat rewrite map_map.
+           apply map_ext_in. intros; solve_length.
+        -- specialize (H14 a0 (Str.const b (Op.false_const)) _ _ _ H12 eq_refl eq_refl).
+           repeat simpl_nth; [| eassumption].
+           eauto.
+      * rewrite concat_map_singl2. assumption.
+    - (* app (reset) *)
+      repeat inv_bind. unfold normalize_exps in H1; repeat inv_bind.
+      assert (length x4 = 1) as Hlength2.
+      { eapply normalize_exp_length in H0... rewrite <- length_typeof_numstreams in H0.
+        rewrite H0. rewrite H10. reflexivity. }
+      repeat singleton_length; subst.
+      eapply normalize_exp_sem in H0...
+      destruct H0 as [H' [Href1 [Hvalid1 [Histst1 [Hsem1 Hsem1']]]]]. inv Hsem1; clear H15.
+      eapply normalize_reset_sem in H2... 2:(destruct Histst1; auto).
+      destruct H2 as [H'' [Href2 [Hvalid2 [Histst2 [Hsem2 Hsem2']]]]].
+      assert (Forall2 (sem_exp G H'' b) l ss) as Hsem'.
+      { repeat rewrite_Forall_forall. eapply sem_exp_refines; [| eauto]. etransitivity... }
+      eapply normalize_exps_sem in H1...
+      destruct H1 as [H''' [Href3 [Hvalid3 [Histst3 [Hsem3 Hsem3']]]]].
+      exists H'''. repeat (split; auto).
+      + repeat (etransitivity; eauto).
+      + right. eexists; split...
+        apply Sreset with (ss:=(concat (List.map (fun x => List.map (fun x => [x]) x) ss))) (rs:=rs) (bs:=bs); eauto.
+        * apply Forall2_concat.
+          repeat rewrite_Forall_forall; solve_length;
+            specialize (H1 a (List.map (fun _ => (Str.const b (Op.false_const))) b0) _ _ _ H19 eq_refl eq_refl);
+            repeat rewrite_Forall_forall; simpl_length.
+          -- rewrite <- map_nth.
+             rewrite <- (map_nth (length (A:=_)) (List.map _ ss)). f_equal; solve_length.
+             repeat rewrite map_map.
+             apply map_ext_in. intros; solve_length.
+          -- specialize (H21 a0 (Str.const b (Op.false_const)) _ _ _ H20 eq_refl eq_refl).
+             repeat simpl_nth; [| eassumption].
+             eauto.
+        * eapply sem_exp_refines...
+        * rewrite concat_map_singl2. assumption.
+      + repeat rewrite Forall_app.
+        repeat split; solve_forall; (eapply sem_equation_refines; [| eauto]); eauto.
+        etransitivity...
+  Qed.
+
+  Corollary map_bind2_normalize_rhs_sem : forall G vars b keep_fby es H vs es' eqs' st st',
+      Forall (wt_exp G vars) es ->
+      Forall2 (sem_exp G H b) es vs ->
+      valid_after vars st ->
+      hist_st G vars b H st ->
+      map_bind2 (normalize_rhs keep_fby) es st = (es', eqs', st') ->
+      (exists H',
+          Env.refines eq H H' /\
+          valid_after vars st' /\
+          hist_st G vars b H' st' /\
+          Forall2 (fun es' vs =>
+                     Forall2 (fun e v => sem_exp G H' b e [v]) es' vs \/
+                     exists e', (es' = [e'] /\ sem_exp G H' b e' vs)) es' vs /\
+          Forall (sem_equation G H' b) (concat eqs')).
+  Proof with eauto.
+    induction es; intros H vs es' eqs' st st' Hwt Hsem Hvalid Histst Hmap;
+      simpl in *; repeat inv_bind.
+    - exists H; simpl. inv Hsem. repeat (split; auto).
+    - inv Hwt. inv Hsem.
+      eapply normalize_rhs_sem in H0...
+      destruct H0 as [H' [Href1 [Hvalid1 [Histst1 [Hsem1 Hsem1']]]]].
+      assert (Forall2 (sem_exp G H' b) es l') as Hsem'.
+      { repeat rewrite_Forall_forall. eapply sem_exp_refines... }
+      eapply IHes in H1... clear IHes.
+      destruct H1 as [H'' [Href2 [Hvalid2 [Histst2 [Hsem2 Hsem2']]]]].
+      exists H''. repeat (split; auto); simpl.
+      + etransitivity...
+      + constructor...
+        destruct Hsem1.
+        * left. repeat rewrite_Forall_forall. eapply sem_exp_refines...
+        * right. destruct H0 as [e' [? H0]]; subst.
+          exists e'. split... eapply sem_exp_refines...
+      + apply Forall_app. split...
+        solve_forall. eapply sem_equation_refines...
+  Qed.
+
+  Corollary normalize_rhss_sem : forall G vars b keep_fby es H vs es' eqs' st st',
+      Forall (wt_exp G vars) es ->
+      Forall2 (sem_exp G H b) es vs ->
+      valid_after vars st ->
+      hist_st G vars b H st ->
+      normalize_rhss keep_fby es st = (es', eqs', st') ->
+      (exists H',
+          Env.refines eq H H' /\
+          valid_after vars st' /\
+          hist_st G vars b H' st' /\
+          Forall (fun '(e, v) => sem_exp G H' b e v)
+                 (combine_for_numstreams es' (concat vs)) /\
+          Forall (sem_equation G H' b) eqs').
+  Proof with eauto.
+    intros G vars b keep_fby es H vs es' eqs' st st' Hwt Hsem Hvalid Histst Hnorm.
+    assert (Forall (wt_exp G (vars++Typ.st_tys st')) es') as Hwt'.
+    { eapply Typ.normalize_rhss_wt_exp in Hnorm... }
+    unfold normalize_rhss in *.
+    repeat inv_bind.
+    eapply map_bind2_normalize_rhs_sem in H0...
+    destruct H0 as [H' [Href1 [Hvalid1 [Histst1 [Hsem1 Hsem1']]]]].
+    exists H'. repeat (split; auto).
+    clear Hsem. induction Hsem1; simpl...
+    simpl. destruct H0.
+    - induction H0; simpl in *...
+      inv Hwt'.
+      assert (numstreams x = 1) as Hnumstreams.
+      { eapply sem_exp_numstreams in H0... }
+      constructor.
+      + rewrite Hnumstreams; simpl...
+      + rewrite Hnumstreams; simpl...
+    - destruct H0 as [? [? H0]]; subst; simpl in *.
+      inv Hwt'.
+      assert (numstreams x1 = length y) as Hnumstreams.
+      { eapply sem_exp_numstreams in H0... }
+      constructor.
+      + rewrite firstn_app...
+      + rewrite skipn_app...
+  Qed.
 
   (** ** Conservation of sem_equation *)
 
+  Fact combine_for_numstreams_length {V} : forall es (vs : list V),
+      length (combine_for_numstreams es vs) = length es.
+  Proof.
+    induction es; intros vs; simpl; auto.
+  Qed.
+
+  Fact combine_for_numstreams_fst_split {V} : forall es (vs : list V),
+      fst (split (combine_for_numstreams es vs)) = es.
+  Proof.
+    induction es; intros vs; simpl.
+    - reflexivity.
+    - destruct (split _) eqn:Hsplit; simpl.
+      assert (fst (l, l0) = es).
+      { rewrite <- Hsplit; auto. }
+      simpl in H. f_equal; auto.
+  Qed.
+
+  Fact combine_for_numstreams_numstreams {V} : forall es (vs : list V),
+      length vs = length (annots es) ->
+      Forall (fun '(e, v) => numstreams e = length v) (combine_for_numstreams es vs).
+  Proof with eauto.
+    induction es; intros vs Hlen; simpl in *...
+    rewrite app_length in Hlen.
+    rewrite length_annot_numstreams in Hlen.
+    constructor...
+    - rewrite firstn_length.
+      symmetry. apply Nat.min_l.
+      omega.
+    - apply IHes.
+      rewrite skipn_length.
+      omega.
+  Qed.
+
+  Fact combine_for_numstreams_nth_2 {V1 V2} : forall es (v1s : list V1) (v2s : list V2) n n0 e v1 v2 d1 d2 de1 de2,
+      length v1s = length (annots es) ->
+      length v2s = length (annots es) ->
+      n < length es ->
+      n0 < length v1 ->
+      nth n (combine_for_numstreams es v1s) de1 = (e, v1) ->
+      nth n (combine_for_numstreams es v2s) de2 = (e, v2) ->
+      exists n',
+        (n' < length v1s /\
+         nth n' v1s d1 = nth n0 v1 d1 /\
+         nth n' v2s d2 = nth n0 v2 d2).
+  Proof with eauto.
+    induction es; intros v1s v2s n n0 e v1 v2 d1 d2 de1 de2 Hlen1 Hlen2 Hn Hn0 Hnth1 Hnth2;
+      simpl in *; try omega.
+    rewrite app_length in *. rewrite length_annot_numstreams in *.
+    destruct n.
+    - inv Hnth1; inv Hnth2.
+      rewrite firstn_length in Hn0; rewrite Nat.min_glb_lt_iff in Hn0; destruct Hn0.
+      exists n0. repeat split...
+      + rewrite nth_firstn_1...
+      + rewrite nth_firstn_1...
+    - apply lt_S_n in Hn.
+      eapply IHes in Hn. 4,5,6:eauto.
+      + destruct Hn as [n' [Hlen' [Hnth1' Hnth2']]].
+        exists (n'+(numstreams a)).
+        repeat split.
+        * rewrite skipn_length in Hlen'. omega.
+        * rewrite nth_skipn in Hnth1'...
+        * rewrite nth_skipn in Hnth2'...
+      + rewrite skipn_length. omega.
+      + rewrite skipn_length. omega.
+  Qed.
+
   Fact normalize_equation_sem : forall G vars H b to_cut equ eqs' st st',
       wt_equation G vars equ ->
-      before_st (List.map fst vars) st ->
-      Env.dom H ((List.map fst vars)++(st_ids st)) ->
       sem_equation G H b equ ->
+      valid_after vars st ->
+      hist_st G vars b H st ->
       normalize_equation to_cut equ st = (eqs', st') ->
       (exists H', Env.refines eq H H' /\
-             Env.dom H' ((List.map fst vars)++(st_ids st')) /\
+             valid_after vars st' /\
+             hist_st G vars b H' st' /\
              Forall (sem_equation G H' b) eqs').
-  Proof.
-  Admitted.
+  Proof with eauto.
+    intros G vars H b to_cut equ eqs' st st' Hwt Hsem Hvalid Histst Hnorm.
+    unfold normalize_equation in Hnorm.
+    destruct equ as [xs es]. inv Hwt. inv Hsem.
+    repeat inv_bind.
+    specialize (normalize_rhss_annots _ _ _ _ _ _ _ _ H0 H2) as Hannots.
+    eapply normalize_rhss_sem in H2...
+    destruct H2 as [H' [Href1 [Hvalid1 [Histst1 [Hsem1 Hsem1']]]]].
+    exists H'. repeat (split; eauto).
+    apply Forall_app. split...
+    clear Hsem1'.
+    repeat rewrite_Forall_forall.
+    destruct x1. repeat simpl_In. inv H7.
+    assert (HIn := H8).
+    eapply In_nth with (d:=(hd_default [], [])) in H8. destruct H8 as [n [Hn Hnth]].
+    rewrite combine_for_numstreams_length in Hn. rewrite <- (combine_for_numstreams_length _ (concat ss)) in Hn.
+    assert (HIn' := Hn).
+    apply nth_In with (d:=(hd_default [], [])) in HIn'.
+    specialize (Hsem1 _ HIn').
+    destruct (nth _ _ _) eqn:Hnth' in Hsem1. rewrite Hnth' in HIn'.
+    assert (e = e0) as Hee0.
+    { rewrite split_nth in Hnth; inv Hnth.
+      rewrite split_nth in Hnth'; inv Hnth'.
+      repeat rewrite combine_for_numstreams_fst_split. reflexivity. } subst.
+    apply Seq with (ss:=[l0]).
+    + repeat constructor...
+    + simpl. rewrite app_nil_r.
+      repeat rewrite_Forall_forall.
+      * rewrite typesof_annots in H1. rewrite map_length in H1. rewrite <- Hannots in H1.
+        replace (length l) with (numstreams e0). replace (length l0) with (numstreams e0). reflexivity.
+        { rewrite H2 in H1. apply combine_for_numstreams_numstreams in H1.
+          rewrite Forall_forall in H1. apply H1 in HIn'... }
+        { apply combine_for_numstreams_numstreams in H1.
+          rewrite Forall_forall in H1. apply H1 in HIn... }
+      * eapply sem_var_refines...
+        specialize (combine_for_numstreams_nth_2 x xs (concat ss) n n0 e0 l l0
+                                                 a b0 (hd_default [], []) (hd_default [], [])) as Hcomb.
+        apply Hcomb in H7. clear Hcomb.
+        2,3:(rewrite typesof_annots in H1; rewrite <- Hannots in H1; rewrite map_length in H1).
+        2:eapply H1. 2:(rewrite H2 in H1; eapply H1).
+        3,4:auto.
+        2:(rewrite combine_for_numstreams_length in Hn; auto).
+        destruct H7 as [n' [Hlen' [Hnth1' Hnth2']]].
+        eapply H3...
+  Qed.
 
   Corollary normalize_equations_sem : forall G vars b to_cut eqs H eqs' st st',
       Forall (wt_equation G vars) eqs ->
       Forall (sem_equation G H b) eqs ->
-      before_st (List.map fst vars) st ->
-      Env.dom H ((List.map fst vars)++(st_ids st)) ->
+      valid_after vars st ->
+      hist_st G vars b H st ->
       normalize_equations to_cut eqs st = (eqs', st') ->
       (exists H', Env.refines eq H H' /\
-             Env.dom H' ((List.map fst vars)++(st_ids st')) /\
              Forall (sem_equation G H' b) eqs').
   Proof with eauto.
-    induction eqs; intros H eqs' st st' Hwt Hsem Hbef Hdome Hnorm;
+    induction eqs; intros H eqs' st st' Hwt Hsem Hvalid Hdome Hnorm;
       inv Hwt; inv Hsem; simpl in Hnorm; repeat inv_bind.
     - exists H...
-    - assert (fresh_st_follows st x0)...
-      eapply normalize_equation_sem in H0... destruct H0 as [H' [Href1 [Hdom1 Hsem1]]].
+    - eapply normalize_equation_sem in H0...
+      destruct H0 as [H' [Href1 [Hvalid1 [Histst1 Hsem1]]]].
       assert (Forall (sem_equation G H' b) eqs) by (solve_forall; eapply sem_equation_refines; eauto).
-      eapply before_st_follows in Hbef...
-      specialize (IHeqs _ _ _ _ H3 H0 Hbef Hdom1 H1). destruct IHeqs as [H'' [Href2 [Hdom2 Hsem2]]].
+      eapply IHeqs in H1...
+      destruct H1 as [H'' [Href Hsem2]].
       exists H''. repeat split...
       + etransitivity...
       + eapply Forall_app. split...
@@ -606,3 +1389,6 @@ Module CorrectnessFun
   Include CORRECTNESS Ids Op OpAux Str Syn Typ Lord Sem Norm.
   Module Typing := NTypingFun Ids Op OpAux Syn Typ Norm.
 End CorrectnessFun.
+
+(* H sem_node G n
+   H' \ dom H' (in++out++vars) /\ refines eq H' H *)
